src/SealedSubst.v
@@ -1,0 +1,80 @@
+Require Import List.
+Require Import Relations.
+Require Import ExtLib.Data.Set.ListSet.
+Require Import ExtLib.Tactics.Consider.
+Require Import ExtLib.Tactics.Injection.
+Require Import MirrorCore.TypesI.
+Require Import MirrorCore.ExprI.
+Require Import MirrorCore.EnvI.
+Require Import MirrorCore.Subst.
+
+Set Implicit Arguments.
+Set Strict Implicit.
+
+Section sealed.
+  Variable expr : Type.
+  Variable lsubst : Type.
+  Context {Subst_lsubst : Subst lsubst expr}.
+  Let uvar : Type := nat.
+
+  Record seal_subst : Type := SealedSubst
+  { allowed : uvar -> bool
+  ; subst : lsubst
+  }.
+
+  Instance Injective_seal_subst a b c d
+  : Injective ({| allowed := a ; subst := b |} =
+               {| allowed := c ; subst := d |}) :=
+  { result := a = c /\ b = d }.
+  Proof.
+    abstract (inversion 1; intuition).
+  Defined.
+
+  Instance Subst_seal_subst : Subst seal_subst expr :=
+  { set := fun u e s =>
+             match s with
+               | {| allowed := allow ; subst := subst |} =>
+                 if allow u then
+                   match set u e subst with
+                     | None => None
+                     | Some s => Some {| allowed := allow ; subst := s |}
+                   end
+                 else
+                   None
+             end
+  ; lookup := fun u s => lookup u s.(subst)
+  ; subst := fun s e => Subst.subst s.(subst) e
+  }.
+
+  Variable typ : Type.
+  Variable typD : list Type -> typ -> Type.
+  Context {Expr_expr : Expr typD expr}.
+  Context {SubstOk_lsubst : @SubstOk _ _ _ _ Expr_expr Subst_lsubst}.
+
+  Instance SubstOk : SubstOk Expr_expr Subst_seal_subst :=
+  { substD := fun us vs s => substD us vs s.(subst)
+  ; WellTyped_subst := fun tus tvs s => WellTyped_subst tus tvs s.(subst)
+  }.
+  Proof.
+    destruct s; simpl; eauto using substD_subst.
+    destruct s; simpl; eauto using substD_subst, substD_lookup.
+    destruct s; simpl; eauto using substD_subst, substD_lookup, WellTyped_subst_lookup, WellTyped_subst_set, substD_set.
+    { destruct s; destruct s'; simpl; eauto using substD_subst, substD_lookup, WellTyped_subst_lookup, WellTyped_subst_set, substD_set.
+      intros. destruct (allowed0 uv); try congruence.
+      consider (set uv e subst0); intros; inv_all; subst; try congruence;
+      eauto using WellTyped_subst_set. }
+    { destruct s; destruct s'; simpl; intros.
+      destruct (allowed0 uv); try congruence; inv_all; subst.
+      consider (set uv e subst0); try congruence; intros; inv_all; subst;
+      eauto using substD_set. }
+  Defined.
+
+  Definition seal : (uvar -> bool) -> lsubst -> seal_subst := SealedSubst.
+
+  Definition exclude (ls : list uvar) : lsubst -> seal_subst :=
+    seal (fun u => negb (List.anyb (EqNat.beq_nat u) ls)).
+
+  Definition allow (ls : list uvar) : lsubst -> seal_subst :=
+    seal (fun u => List.anyb (EqNat.beq_nat u) ls).
+
+End sealed.
